src/crdts/MVregisterSingle_impl_valid.thy
@@ -1,39 +1,9 @@
-theory MVregisterSingle
-imports induction helper convergence 
+theory MVregisterSingle_impl_valid
+imports 
+MVregisterSingle_impl
+"../framework/induction" 
+"../framework/helper" 
 begin
-
-datatype 'a updateArgs = Assign 'a
-type_synonym 'a returnType = "'a set"
-
-definition mvRegisterSpec :: "('a updateArgs, unit, 'a returnType) crdtSpecification" where
-"mvRegisterSpec H _ = {(x). \<exists>e\<in>allUpdates H. updArgs(e) = Assign x \<and> \<not>(\<exists>f\<in>allUpdates H. e \<prec> f)}"
-
-type_synonym 'a payload = "versionVector \<times> ('a \<times> versionVector) set"
-
-fun update :: "'a updateArgs \<Rightarrow> replicaId \<Rightarrow> 'a payload \<Rightarrow> 'a payload" where
-"update (Assign x) r (V,S) = (incVV r V, S \<union> {(x, incVV r V)})"
-
-fun getValue :: "unit \<Rightarrow> 'a payload \<Rightarrow> 'a set" where
-"getValue _ (V,S) = fst ` {(x,v)\<in>S. \<not>(\<exists>(x',v')\<in>S. v < v')}"
-
-definition mvRegister where
-"mvRegister = \<lparr> 
-      t_compare = (\<lambda>x y. fst x \<le> fst y \<and> snd x \<subseteq> snd y),
-      t_merge   = (\<lambda>x y. (sup (fst x) (fst y), snd x \<union> snd y)),
-      t_initial = (vvZero, {}),
-      t_update  = update,
-      t_query   = getValue       
-  \<rparr>"
-
-lemma crdtProps: "crdtProperties mvRegister (\<lambda>H pl. True)"
-apply (rule unfoldCrdtProperties)
-apply (auto simp add: mvRegister_def)
-apply (case_tac args, auto)
-apply (metis incVVGreaterEq)
-apply (case_tac args, auto)
-apply (metis sup.commute)
-done
-
 
 definition mvRegisterInvariant :: "('a updateArgs) updateHistory \<Rightarrow> 'a payload \<Rightarrow> bool" where
 "mvRegisterInvariant H pl = (
