src/crdts/PNCounter_impl_valid.thy
@@ -1,43 +1,9 @@
-theory PNCounter
+theory PNCounter_impl_valid
 imports 
+PNCounter_impl
 "../framework/induction"
-"../framework/helper" 
-"../framework/convergence" 
+"../framework/helper"  
 begin
-
-type_synonym payload = "(replicaId \<Rightarrow> int) \<times> (replicaId \<Rightarrow> int)"
-
-fun update :: "int \<Rightarrow> replicaId \<Rightarrow> payload \<Rightarrow> payload" where
- "update x r (p,n) = (if x \<ge> 0 then (p(r:=p r + x), n) else (p, n(r:=n r - x)))"
-
-fun getValue :: "unit \<Rightarrow> payload \<Rightarrow> int" where
-"getValue _ (p,n) = ((\<Sum>r\<in>UNIV. p r) - (\<Sum>r\<in>UNIV. n r))"
-
-definition pnCounter where
-"pnCounter = \<lparr> 
-      t_compare = (\<lambda>x y. \<forall>r. fst x r \<le> fst y r \<and> snd x r \<le> snd y r),
-      t_merge   = (\<lambda>x y. (\<lambda>r. max (fst x r) (fst y r), \<lambda>r. max (snd x r) (snd y r))),
-      t_initial = (\<lambda>r. 0, \<lambda>r. 0),
-      t_update  = update,
-      t_query   = getValue       
-  \<rparr>"
-
-
-lemma ORsetSimple_crdtProps: "crdtProperties pnCounter (\<lambda>UH pl. True)"
-apply (rule unfoldCrdtProperties)
-apply (case_tac args)
-apply (auto simp add: pnCounter_def)
-apply (metis order_trans)
-apply (metis order_trans)
-apply (rule ext)
-apply (metis antisym)
-apply (rule ext)
-apply (metis antisym)
-done
-
-
-definition pnCounterSpec :: "(int,unit,int) crdtSpecification" where
-"pnCounterSpec H q = (\<Sum>e\<in>allUpdates H. updArgs(e))"
 
 definition pnCounterInvariant where
 "pnCounterInvariant H pl = (\<forall>r. (fst pl) r = listsum (map updArgs (filter (\<lambda>x. updArgs x \<ge> 0) (H r))) 
