src/crdts/gset_impl_valid.thy
@@ -1,38 +1,9 @@
-theory gset
+theory gset_impl_valid
 imports 
+gset_impl
 "../framework/induction"
 "../framework/helper" 
-"../framework/convergence" 
 begin
-
-
-definition add :: "'a \<Rightarrow> replicaId \<Rightarrow> 'a set \<Rightarrow> 'a set" where
-"add x r = insert x"
-
-definition lookup :: "'a \<Rightarrow> 'a set \<Rightarrow> bool" where
-"lookup x pl = (x\<in>pl)"
-
-definition gSet :: "('a set, 'a, 'a, bool) stateBasedType" where
-"gSet = \<lparr> 
-      t_compare = op\<subseteq>,
-      t_merge   = op\<union>,
-      t_initial = {},
-      t_update  = add,
-      t_query   = lookup      
-  \<rparr>"
-
-(* convergence *)
-lemma ORsetSimple_crdtProps: "crdtProperties gSet (\<lambda>UH pl. True)"
-apply (rule unfoldCrdtProperties)
-apply (auto simp add: gSet_def add_def)
-done
-
-
-(* specification *)
-
-(* x is in the set when there is an add operation *)
-definition gSetSpec :: "('a,'a,bool) crdtSpecification" where
-"gSetSpec H x = (\<exists>e\<in>allUpdates H. updArgs(e) = x)"
 
 definition gSetInvariant where
 "gSetInvariant H pl = (\<forall>x. x\<in> pl \<longleftrightarrow> (\<exists>e\<in>allUpdates H. updArgs(e) = x))"
