src/all.thy
@@ -13,44 +13,75 @@ imports Main
 "framework/helper"
 
 (* case studies *)
-"crdts/IncrementOnlyCounter"
-"crdts/PNCounter"
-
-"crdts/gset"
-"crdts/twoPhaseSet"
-"crdts/twoPhaseSet2"
-
-"crdts/ORsetSimple"
-"crdts/ORset"
-"crdts/ORsetOptimized"
-"crdts/ORsetOptimizedConvergence"
-"crdts/ORsetOptimizedValid"
-
-"crdts/MVregisterSimple"
-"crdts/MVregister"
+"crdts/gset_impl"
+"crdts/gset_impl_convergence"
+"crdts/gset_impl_valid"
+"crdts/gset_spec"
+"crdts/IncrementOnlyCounter_impl"
+"crdts/IncrementOnlyCounter_impl_convergence"
+"crdts/IncrementOnlyCounter_impl_valid"
+"crdts/IncrementOnlyCounter_spec"
+"crdts/MVregister2_impl"
+"crdts/MVregister2_impl_convergence"
+"crdts/MVregister2_impl_valid"
+"crdts/MVregister2_spec"
+"crdts/MVregister_impl"
+"crdts/MVregister_impl_convergence"
+"crdts/MVregister_impl_valid"
+"crdts/MVregisterSingle_spec"
+"crdts/MVregisterSingle_impl"
+"crdts/MVregisterSingle_impl_convergence"
+"crdts/MVregisterSingle_impl_valid"
+"crdts/MVregister_spec"
+"crdts/ORset_impl"
+"crdts/ORset_impl_convergence"
+"crdts/ORset_impl_valid"
+"crdts/ORset_optimized"
+"crdts/ORset_optimized_convergence"
+"crdts/ORset_optimized_valid"
+"crdts/ORset_simple"
+"crdts/ORset_simple_convergence"
+"crdts/ORset_simple_valid"
+"crdts/ORset_spec"
+"crdts/PNCounter_impl"
+"crdts/PNCounter_impl_convergence"
+"crdts/PNCounter_impl_valid"
+"crdts/PNCounter_spec"
+"crdts/twoPhaseSet2_impl"
+"crdts/twoPhaseSet2_impl_convergence"
+"crdts/twoPhaseSet2_impl_valid"
+"crdts/twoPhaseSet2_spec"
+"crdts/twoPhaseSet_impl"
+"crdts/twoPhaseSet_impl_convergence"
+"crdts/twoPhaseSet_impl_valid"
+"crdts/twoPhaseSet_spec"
 begin
 
 
 
-
+(* lemma using all important theorems, so that they are not marked as unused *)
 lemma dummyUsage: "True"
-apply (cut_tac IncrementOnlyCounter.crdtProps)
-apply (cut_tac IncrementOnlyCounter.specValid)
-apply (cut_tac MVregister.crdtProps)
-apply (cut_tac MVregisterSimple.crdtProps)
-apply (cut_tac MVregisterSimple.specValid)
-apply (cut_tac ORset.ORsetSimple_crdtProps)
-apply (cut_tac ORset.setSpecValid)
-apply (cut_tac ORsetOptimizedConvergence.ORsetSimple_crdtProps)
-apply (cut_tac ORsetOptimizedValid.setSpecValid)
-apply (cut_tac ORsetSimple.ORsetSimple_crdtProps)
-apply (cut_tac PNCounter.ORsetSimple_crdtProps)
+apply (cut_tac IncrementOnlyCounter_impl_convergence.crdtProps)
+apply (cut_tac IncrementOnlyCounter_impl_valid.specValid)
+apply (cut_tac MVregister_impl_convergence.crdtProps)
+apply (cut_tac MVregister_impl_convergence.crdtProps)
+apply (cut_tac MVregister_impl_valid.specValid)
+apply (cut_tac ORset_impl_convergence.ORsetSimple_crdtProps)
+apply (cut_tac ORset_impl_valid.setSpecValid)
+apply (cut_tac ORset_optimized_convergence.ORsetSimple_crdtProps)
+apply (cut_tac ORset_optimized_valid.setSpecValid)
+apply (cut_tac ORset_simple_convergence.ORsetSimple_crdtProps)
+apply (cut_tac PNCounter_impl_convergence.ORsetSimple_crdtProps)
 apply (cut_tac counterSpecValid)
-apply (cut_tac gset.ORsetSimple_crdtProps)
-apply (cut_tac twoPhaseSet.ORsetSimple_crdtProps)
-apply (cut_tac twoPhaseSet2.ORsetSimple_crdtProps)
+apply (cut_tac gset_impl_convergence.ORsetSimple_crdtProps)
+apply (cut_tac twoPhaseSet_impl_convergence.ORsetSimple_crdtProps)
+apply (cut_tac twoPhaseSet2_impl_convergence.ORsetSimple_crdtProps)
 
-apply (auto simp add: IncrementOnlyCounter.crdtProps) 
+apply (cut_tac MVregister2_impl_convergence.crdtProps)
+apply (cut_tac MVregisterSingle_impl_convergence.crdtProps)
+apply (cut_tac MVregisterSingle_impl_valid.specValid)
+
+apply (auto simp add: IncrementOnlyCounter_impl_convergence.crdtProps) 
 done
 
 lemma dummyUsage2: "False \<Longrightarrow> True"
