src/crdts/IncrementOnlyCounter_impl.thy
@@ -1,0 +1,24 @@
+theory IncrementOnlyCounter_impl
+imports 
+IncrementOnlyCounter_spec
+"../framework/systemModel" 
+begin
+
+
+definition increment :: "unit \<Rightarrow> replicaId \<Rightarrow> versionVector \<Rightarrow> versionVector" where
+"increment _ r = incVV r"
+
+definition getValue :: "unit \<Rightarrow> versionVector \<Rightarrow> nat" where
+"getValue _ v =  (\<Sum>r\<in>UNIV. v\<guillemotright>r)"
+
+definition incrementOnlyCounter :: "(versionVector, unit, unit, nat) stateBasedType" where
+"incrementOnlyCounter = \<lparr> 
+      t_compare = op\<le>,
+      t_merge   = sup,
+      t_initial = vvZero,
+      t_update  = increment,
+      t_query   = getValue       
+  \<rparr>"
+
+end
+
