src/crdts/IncrementOnlyCounter_impl_convergence.thy
@@ -1,0 +1,15 @@
+theory IncrementOnlyCounter_impl_convergence
+imports 
+IncrementOnlyCounter_impl
+"../framework/convergence"
+begin
+
+lemma crdtProps: "crdtProperties incrementOnlyCounter (\<lambda>UH pl. True)"
+apply (rule unfoldCrdtProperties)
+apply (case_tac args)
+apply (auto simp add: incrementOnlyCounter_def increment_def)
+apply (simp add: incVVGreaterEq)
+apply (simp add: sup_commute)
+done
+
+end
