src/crdts/MVregister2_impl_valid.thy
@@ -1,0 +1,15 @@
+theory MVregister2_impl_valid
+imports 
+MVregister2_impl
+begin
+
+definition mvRegisterInvariant  where
+"mvRegisterInvariant H pl = ((\<forall>x c. (Some x, c)\<in>pl 
+  \<longleftrightarrow> (\<exists>r l v. x\<in>set l \<and> (v, Assign l)\<in>set(H r)
+    \<and> (\<forall>rr. c\<guillemotright>rr = length (filter (\<lambda>e. updArgs e \<noteq> Assign [] \<and> updVersion e \<le> v ) (H rr)))
+    \<and> \<not>(\<exists>l' vv. l' \<noteq> [] \<and> vv>v \<and> (vv, Assign l')\<in>allUpdates H)))
+  \<and> (\<forall>x. (None,x)\<in>pl \<longleftrightarrow> x=vvZero \<and> H = (\<lambda>r. [])))"
+
+(* no proof *)
+
+end
