src/crdts/MVregister_impl.thy
@@ -1,0 +1,23 @@
+theory MVregister_impl
+imports 
+MVregister_spec
+begin
+
+type_synonym 'a payload = "versionVector \<times> ('a list \<times> versionVector) set"
+
+fun update :: "'a updateArgs \<Rightarrow> replicaId \<Rightarrow> 'a payload \<Rightarrow> 'a payload" where
+"update (Assign l) r (V,S) = (incVV r V, S \<union> {(l, incVV r V)})"
+
+fun getValue :: "unit \<Rightarrow> 'a payload \<Rightarrow> ('a \<times> versionVector )set" where
+"getValue _ (V,S) = {(x,v). \<exists>l. x\<in>set l \<and> (l,v)\<in>S \<and> (\<forall>vv\<in>snd`S. \<not>v<vv)}"
+
+definition mvRegister where
+"mvRegister = \<lparr> 
+      t_compare = (\<lambda>x y. fst x \<le> fst y \<and> snd x \<subseteq> snd y),
+      t_merge   = (\<lambda>x y. (sup (fst x) (fst y), snd x \<union> snd y)),
+      t_initial = (vvZero, {}),
+      t_update  = update,
+      t_query   = getValue       
+  \<rparr>"
+
+end
