src/crdts/MVregister_impl_convergence.thy
@@ -1,0 +1,17 @@
+theory MVregister_impl_convergence
+imports 
+MVregister_impl
+"../framework/convergence" 
+begin
+
+
+lemma crdtProps: "crdtProperties mvRegister (\<lambda>H pl. True)"
+apply (rule unfoldCrdtProperties)
+apply (auto simp add: mvRegister_def)
+apply (case_tac args, auto)
+apply (metis incVVGreaterEq)
+apply (case_tac args, auto)
+apply (metis sup.commute)
+done
+
+end
