src/crdts/ORset_simple.thy
@@ -1,0 +1,58 @@
+theory ORset_simple
+imports ORset_spec 
+"../framework/induction"
+"../framework/helper" 
+"../framework/convergence" 
+begin
+
+(* simpler version of OR-set (but takes more space, queries take more time)
+Here all sets are increasing, so semilattice properties do not have to be shown.
+Also no invariant is necessary.
+*)
+type_synonym 'a payload = "('a \<times> versionVector) set \<times> ('a \<times> versionVector) set \<times> versionVector"
+
+
+abbreviation elements :: "'a payload \<Rightarrow> ('a \<times> versionVector) set" where
+"elements x \<equiv> fst x"
+
+abbreviation tombstones :: "'a payload \<Rightarrow> ('a \<times> versionVector) set" where
+"tombstones x \<equiv> fst (snd x)"
+
+abbreviation versionVec :: "'a payload \<Rightarrow> versionVector" where
+"versionVec x \<equiv> snd (snd x)"
+
+
+definition add :: "replicaId \<Rightarrow> 'a payload \<Rightarrow> 'a \<Rightarrow> 'a payload" where 
+"add myId pl e = (let vv = incVV myId (versionVec pl) in 
+      (elements pl \<union> {(e,vv)}, tombstones pl, vv))"
+
+definition remove :: "replicaId \<Rightarrow> 'a payload \<Rightarrow> 'a \<Rightarrow> 'a payload" where
+"remove myId pl e = (let R = {(e',n). (e',n)\<in>elements pl \<and> e'=e} in 
+    (elements pl, tombstones pl \<union> R, incVV myId (versionVec pl)))"
+
+definition contains :: "'a payload \<Rightarrow> 'a \<Rightarrow> bool" where
+"contains pl e = (\<exists>n. (e,n)\<in>elements pl \<and> (e,n)\<notin>tombstones pl)"
+
+definition getElements :: "'a payload \<Rightarrow> 'a set" where
+"getElements pl = {e. contains pl e}"
+
+fun update :: "'a updateArgs \<Rightarrow> replicaId \<Rightarrow> 'a payload \<Rightarrow> 'a payload" where
+  "update (Add e) r pl = add r pl e"
+| "update (Remove e) r pl = remove r pl e"
+
+fun getValue :: "'a queryArgs \<Rightarrow> 'a payload \<Rightarrow> 'a result" where
+  "getValue (Contains e) pl = ContainsResult (contains pl e)"
+| "getValue (GetElements) pl = GetElementsResult (getElements pl)"
+
+definition ORsetSimple where
+"ORsetSimple = \<lparr> 
+      t_compare = (\<lambda>A B. elements A \<subseteq> elements B \<and> tombstones A \<subseteq> tombstones B \<and> versionVec A \<le> versionVec B),
+      t_merge   = (\<lambda>A B. (elements A \<union> elements B, tombstones A \<union> tombstones B, sup (versionVec A) (versionVec B))),
+      t_initial = ({}, {}, vvZero),
+      t_update  = update,
+      t_query   = getValue       
+  \<rparr>"
+
+
+end
+
