src/crdts/gset_impl.thy
@@ -1,0 +1,26 @@
+theory gset_impl
+imports 
+gset_spec
+"../framework/induction"
+"../framework/helper" 
+"../framework/convergence" 
+begin
+
+
+definition add :: "'a \<Rightarrow> replicaId \<Rightarrow> 'a set \<Rightarrow> 'a set" where
+"add x r = insert x"
+
+definition lookup :: "'a \<Rightarrow> 'a set \<Rightarrow> bool" where
+"lookup x pl = (x\<in>pl)"
+
+definition gSet :: "('a set, 'a, 'a, bool) stateBasedType" where
+"gSet = \<lparr> 
+      t_compare = op\<subseteq>,
+      t_merge   = op\<union>,
+      t_initial = {},
+      t_update  = add,
+      t_query   = lookup      
+  \<rparr>"
+
+end
+
