src/crdts/gset_impl_convergence.thy
@@ -1,0 +1,14 @@
+theory gset_impl_convergence
+imports 
+gset_impl
+"../framework/convergence" 
+begin
+
+lemma ORsetSimple_crdtProps: "crdtProperties gSet (\<lambda>UH pl. True)"
+apply (rule unfoldCrdtProperties)
+apply (auto simp add: gSet_def add_def)
+done
+
+
+end
+
