src/crdts/gset_spec.thy
@@ -1,0 +1,14 @@
+theory gset_spec
+imports 
+"../framework/induction"
+"../framework/helper" 
+"../framework/convergence" 
+begin
+
+(* x is in the set when there is an add operation *)
+definition gSetSpec :: "('a,'a,bool) crdtSpecification" where
+"gSetSpec H x = (\<exists>e\<in>allUpdates H. updArgs(e) = x)"
+
+
+end
+
