src/crdts/twoPhaseSet2_impl_convergence.thy
@@ -1,0 +1,15 @@
+theory twoPhaseSet2_impl_convergence
+imports 
+twoPhaseSet2_impl
+"../framework/convergence" 
+begin
+
+lemma ORsetSimple_crdtProps: "crdtProperties twoPhaseSet (\<lambda>UH pl. True)"
+apply (rule unfoldCrdtProperties)
+apply (auto simp add: twoPhaseSet_def)
+apply (case_tac args, auto)+
+done
+
+
+end
+
