src/crdts/twoPhaseSet2_impl_valid.thy
@@ -1,0 +1,47 @@
+theory twoPhaseSet2_impl_valid
+imports 
+twoPhaseSet2_impl
+"../framework/induction"
+"../framework/helper"  
+begin
+
+
+definition Inv where
+"Inv H pl = (\<forall>x. (x\<in>fst pl \<longleftrightarrow> (\<exists>e\<in>allUpdates H. updArgs(e) = Add x)) 
+  \<and> (x\<in>snd pl \<longleftrightarrow> (\<exists>e\<in>allUpdates H. updArgs(e) = Remove x \<and> (\<exists>f\<in>allUpdates H. updArgs(f) = Add(x) \<and> f \<prec> e))))"
+
+lemma "crdtSpecificationValid twoPhaseSet twoPhaseSetSpec"
+apply (rule_tac Inv="Inv" in showCrdtSpecificationValid)
+(* show that invariant implies spec *)
+apply (simp add: twoPhaseSet_def twoPhaseSetSpec_def Inv_def invariantImpliesSpec_def)
+
+
+(* show that invariant is maintained *)
+apply (auto simp add: updateHistoryInvariant_all_def)
+
+(* initial*)
+apply (auto simp add: updateHistoryInvariant_initial_def)
+apply (simp add: Inv_def twoPhaseSet_def)
+
+(* merge *) 
+apply (auto simp add: updateHistoryInvariant_merge_def)
+apply (simp add: Inv_def twoPhaseSet_def)
+apply auto
+apply (drule_tac x=x in spec) 
+apply (drule_tac x=x in spec)
+apply (metis consistentHistoriesHappensBefore2 fst_conv snd_conv)
+apply (metis (hide_lams, no_types) consistentHistoriesHappensBefore fst_conv snd_conv)
+
+(* update *)
+apply (auto simp add: updateHistoryInvariant_update_def)
+apply (simp add: Inv_def twoPhaseSet_def)
+apply (case_tac args)
+apply auto
+apply (metis laterVersionNotInAllUpdates_incVV)
+apply (metis fst_conv snd_conv versionIsTopGreaterHistory2_incVV)
+done
+
+
+
+end
+
