src/crdts/twoPhaseSet_impl.thy
@@ -1,0 +1,25 @@
+theory twoPhaseSet_impl
+imports 
+twoPhaseSet_spec
+begin
+
+type_synonym 'a payload = "'a set \<times> 'a set"
+
+fun update :: "'a updateArgs \<Rightarrow> replicaId \<Rightarrow> 'a payload \<Rightarrow> 'a payload" where
+  "update (Add x) r (E,T) = (insert x E, T)"
+| "update (Remove x) r (E,T) = (E, insert x T)"
+
+fun lookup :: "'a \<Rightarrow> 'a payload \<Rightarrow> bool" where
+"lookup x (E,T) = (x\<in>E \<and> x\<notin>T)"
+
+definition twoPhaseSet :: "('a payload, 'a updateArgs, 'a, bool) stateBasedType" where
+"twoPhaseSet = \<lparr> 
+      t_compare = (\<lambda>x y. fst x \<subseteq> fst y \<and> snd x \<subseteq> snd y),
+      t_merge   = (\<lambda>x y. (fst x \<union> fst y, snd x \<union> snd y)),
+      t_initial = ({},{}),
+      t_update  = update,
+      t_query   = lookup      
+  \<rparr>"
+
+end
+
