src/crdts/twoPhaseSet_spec.thy
@@ -1,0 +1,14 @@
+theory twoPhaseSet_spec
+imports 
+"../framework/specifications"
+begin
+
+datatype 'a updateArgs = Add 'a | Remove 'a
+
+(* x is in the set when there is an add operation and no remove operation *)
+definition twoPhaseSetSpec :: "('a updateArgs,'a,bool) crdtSpecification" where
+"twoPhaseSetSpec H x = (\<exists>e\<in>allUpdates H. updArgs(e) = Add x \<and> \<not>(\<exists>e\<in>allUpdates H. updArgs(e) = Remove x))"
+
+
+end
+
